	\begin{center}
		\begin{multicols}{3}
			\ \linebreak
			
			\begin{align*}
			&\ \text{S}\circ\text{T}(\sigma(m))\\
			=&\ \text{S}(\sigma(m)+1)\\
			=&\ -(\sigma(m)+1)\\
			=&\ -\sigma(m)-1
			\end{align*}
			
			\underline{S y T no conmutan:}
			
			\begin{align*}
			&\ \text{T}\circ\text{S}(\sigma(m))\\
			=&\ \text{T}(-\sigma(m))\\
			=&\ -\sigma(m)+1
			\end{align*}			
			
			\ \linebreak
			
			\begin{align*}
			&\ \text{S}\circ\text{T}^{-1}(\sigma(m))\\
			=&\ \text{S}(\sigma(m)-1)\\
			=&\ -(\sigma(m)-1)\\
			=&\ -\sigma(m)+1
			%=&\ \text{T}\circ\text{S}(\sigma(m))
			\end{align*}
		\end{multicols}
		
		\begin{multicols}{3}
			\ \linebreak
			
			\begin{align*}
			&\ \text{V}\circ\text{C}(\sigma(m))\\
			=&\ \text{V}(\sigma(m+1))\\
			=&\ \sigma(-(m+1))\\
			=&\ \sigma(-m-1)
			\end{align*}
			
			\underline{V y C no conmutan:}
			
			\begin{align*}
			&\ \text{C}\circ\text{V}(\sigma(m))\\
			=&\ \text{C}(\sigma(-m))\\
			=&\ \sigma(-m+1)
			\end{align*}
			
			\ \linebreak
			
			\begin{align*}
			&\ \text{V}\circ\text{C}^{-1}(\sigma(m))\\
			=&\ \text{V}(\sigma(m-1))\\
			=&\ \sigma(-(m-1))\\
			=&\ \sigma(-m+1)
			%=&\ \text{C}\circ\text{V}(\sigma(m))
			\end{align*}
		\end{multicols}
		
		\begin{multicols}{3}
			\begin{align*}
			&\ \text{S}\circ\text{V}(\sigma(m))\\
			=&\ \text{S}(\sigma(-m))\\
			=&\ -\sigma(-m)
			\end{align*}
			
			\underline{S y V conmutan:}
			
			\begin{align*}
			&\ \text{V}\circ\text{S}(\sigma(m))\\
			=&\ \text{V}(-\sigma(m))\\
			=&\ -\sigma(-m)
			\end{align*}
		\end{multicols}
		
		\begin{multicols}{3}
			\begin{align*}
			&\ \text{S}\circ\text{C}(\sigma(m))\\
			=&\ \text{S}(\sigma(m+1))\\
			=&\ -\sigma(m+1)
			\end{align*}
			
			\underline{S y C conmutan:}
			
			\begin{align*}
			&\ \text{C}\circ\text{S}(\sigma(m))\\
			=&\ \text{C}(-\sigma(m))\\
			=&\ -\sigma(m+1)
			\end{align*}
		\end{multicols}
	
		\begin{multicols}{3}
			\begin{align*}
			&\ \text{T}\circ\text{V}(\sigma(m))\\
			=&\ \text{T}(\sigma(-m))\\
			=&\ \sigma(-m)+1
			\end{align*}
			
			\underline{T y V conmutan:}
			
			\begin{align*}
			&\ \text{V}\circ\text{T}(\sigma(m))\\
			=&\ \text{V}(\sigma(m)+1)\\
			=&\ \sigma(-m)+1
			\end{align*}
		\end{multicols}
		
		\begin{multicols}{3}
			\begin{align*}
			&\ \text{T}\circ\text{C}(\sigma(m))\\
			=&\ \text{T}(\sigma(m+1))\\
			=&\ \sigma(m+1)+1
			\end{align*}
			
			\underline{T y C conmutan:}
			
			\begin{align*}
			&\ \text{C}\circ\text{T}(\sigma(m))\\
			=&\ \text{V}(\sigma(m)+1)\\
			=&\ \sigma(m+1)+1
			\end{align*}
		\end{multicols}
	\end{center}